src/tls/HSCrypto.fst
@@ -65,6 +65,7 @@ assume val derive_keys: gxy:CommonDH.secret -> cr:random -> sr:random -> log:byt
 
 
 (* TLS 1.3 *)
+
 assume val derive_handshake_keys: gxy:CommonDH.secret -> log: bytes ->
 				  rd:rid -> wr:rid -> i:id -> ST ((both i) * ms)
   (requires (fun h -> True))
