src/tls/test/TestClient13.fst
@@ -5,18 +5,21 @@ open FStar.HyperHeap
 open Platform.Bytes
 open Platform.Error
 open HandshakeMessages
+open Handshake
 open TLSError
 open TLSInfo
 open TLSConstants
 open TLSInfo
 open StatefulLHAE
+open CoreCrypto
+
+(* FlexRecord *)
 
 let config =
     let sigPref = [CoreCrypto.RSASIG] in
     let hashPref = [Hash CoreCrypto.SHA256] in
     let sigAlgPrefs = sigAlgPref sigPref hashPref in
     let l =         [ TLS_ECDHE_RSA_WITH_AES_128_GCM_SHA256 ] in
-    cut (List.Tot.length l == 7);//this requires 8 unfoldings
     let csn = cipherSuites_of_nameList l in
      {TLSInfo.defaultConfig with
          minVer = TLS_1p3;
@@ -38,11 +41,12 @@ let id = {
       ne_supported_point_formats = None;
       ne_server_names = None;
       ne_signature_algorithms = None;
+      ne_keyShare = None
     };
     writer = Client
   }
 
-let encryptor_TLS12_AES_GCM_128_SHA256 key iv = 
+let encryptor_TLS13_AES_GCM_128_SHA256 key iv = 
   let r = HyperHeap.root in
   let w: writer id =
     let log: st_log_t r id = ralloc r Seq.createEmpty in
@@ -61,7 +65,7 @@ let encryptor_TLS12_AES_GCM_128_SHA256 key iv =
   // StatefulLHAE.writer -> StatefulLHAE.state
   w
 
-let decryptor_TLS12_AES_GCM_128_SHA256 key iv = 
+let decryptor_TLS13_AES_GCM_128_SHA256 key iv = 
   let r = HyperHeap.root in
   let r: reader id =
     let log: st_log_t r id = ralloc r Seq.createEmpty in
@@ -80,8 +84,8 @@ let decryptor_TLS12_AES_GCM_128_SHA256 key iv =
   // StatefulLHAE.reader -> StatefulLHAE.state
   r
 
-let encryptRecord_TLS12_AES_GCM_128_SHA256 w ct plain = 
-  let pv = TLS_1p2 in
+let encryptRecord_TLS13_AES_GCM_128_SHA256 w ct plain = 
+  let pv = TLS_1p3 in
   let text = plain in
   // StatefulPlain.adata id -> bytes
   let ad: StatefulPlain.adata id = StatefulPlain.makeAD id ct in
@@ -96,25 +100,27 @@ let encryptRecord_TLS12_AES_GCM_128_SHA256 w ct plain =
   // FIXME: without the three additional #-arguments below, extraction crashes
   StatefulLHAE.encrypt #id #ad #rg w f
 
-
-let decryptRecord_TLS12_AES_GCM_128_SHA256 rd ct cipher = 
+let decryptRecord_TLS13_AES_GCM_128_SHA256 rd ct cipher = 
   let ad: StatefulPlain.adata id = StatefulPlain.makeAD id ct in
   let (Some d) = StatefulLHAE.decrypt #id #ad rd cipher in
   Content.repr id d
 
 (* We should use Content.mk_fragment |> Content.repr, not Record.makePacket *)
 (* Even better, we should move to TLS.send *)
-
 let makePacket ct ver (data: b:bytes { repr_bytes (length b) <= 2}) =
       abyte 22z
    @| versionBytes ver
    @| bytes_of_int 2 (length data) 
    @| data 
 
-let sendHSRecord tcp pv log hs_msg = 
-  let r = makePacket Content.Handshake pv hs_msg in
+let sendRecord tcp pv ct msg str = 
+  let r = makePacket ct pv msg in
   let Correct _ = Platform.Tcp.send tcp r in
-  log @| hs_msg
+  match ct with
+  | Content.Application_data ->   IO.print_string ("Sending Data("^str^")\n")
+  | Content.Handshake ->   IO.print_string ("Sending HS("^str^")\n")
+  | Content.Change_cipher_spec ->   IO.print_string ("Sending CCS\n")
+  | Content.Alert ->   IO.print_string ("Sending Alert("^str^")\n")
 
 val really_read_rec: bytes -> Platform.Tcp.networkStream -> nat -> optResult string bytes
 let rec really_read_rec prev tcp len = 
@@ -130,152 +136,145 @@ let rec really_read_rec prev tcp len =
       
 let really_read = really_read_rec empty_bytes
 
-val recvHSRecordRec: bytes -> Platform.Tcp.networkStream -> protocolVersion -> kexAlg -> bytes -> (hs_msg * bytes)
-let rec recvHSRecordRec prev tcp pv kex log = 
-//  IO.print_string (Platform.Bytes.print_bytes prev);
-//  IO.print_string ((string_of_int (length prev))^" left from before\n");
+let recvRecord tcp pv = 
   match really_read tcp 5 with 
   | Correct header ->
       match Record.parseHeader header with  
-      | Correct (Content.Handshake,pv,len)  ->
-         IO.print_string ((string_of_int len)^" bytes expected\n");
+      | Correct (ct,pv,len)  ->
          match really_read tcp len  with
-         | Correct payload -> 
-	      let buf = prev @| payload in 
-	      let Correct (rem,hsm) = Handshake.parseHandshakeMessages (Some pv) (Some kex) buf in 
-	      //IO.print_string ((string_of_int (List.Tot.length hsm))^" messages\n");
-	      //IO.print_string ((string_of_int (length rem))^" left\n");
-	      (match hsm with 
-	      | [] -> recvHSRecordRec rem tcp pv kex log 
-	      | [(hs_msg,to_log)] ->  hs_msg, log @| to_log)
+         | Correct payload -> (ct,pv,payload)
 
-let recvHSRecord = recvHSRecordRec empty_bytes
+let makeHSRecord pv hs_msg log =
+  let hs = HandshakeMessages.handshakeMessageBytes pv hs_msg in
+  (string_of_handshakeMessage hs_msg,hs,log@|hs)
 
-let sendAppDataRecord tcp pv msg = 
-  let r = makePacket Content.Application_data pv msg in
-  let Correct _ = Platform.Tcp.send tcp r in
-  ()
+let sendHSRecord tcp pv hs_msg log = 
+  let (str,hs,log) = makeHSRecord pv hs_msg log in
+  sendRecord tcp pv Content.Handshake hs str;
+  log
 
-let sendCCSRecord tcp pv = 
-  let r = makePacket Content.Change_cipher_spec pv HandshakeMessages.ccsBytes in
-  let Correct _ = Platform.Tcp.send tcp r in
-  ()
-  
+let recvHSRecord tcp pv kex log = 
+  let (Content.Handshake,rpv,pl) = recvRecord tcp pv in
+  match Handshake.parseHandshakeMessages (Some pv) (Some kex) pl with
+  | Correct (rem,[(hs_msg,to_log)]) -> 
+     	    (IO.print_string ("Received HS("^(string_of_handshakeMessage hs_msg)^")\n");
+	     (hs_msg,log @| to_log))
+  | Error (x,z) -> IO.print_string (z^"\n"); failwith "error"
+
 let recvCCSRecord tcp pv = 
-  match really_read tcp 5 with 
-  | Correct header ->
-      match Record.parseHeader header with  
-      | Correct (Content.Change_cipher_spec,pv,len)  ->
-         match really_read tcp len  with
-         | Correct cipher -> cipher
-
+  let (Content.Change_cipher_spec,_,ccs) = recvRecord tcp pv in
+  IO.print_string "Received CCS\n";
+  ccs
 
 let recvEncHSRecord tcp pv kex log rd = 
-  match really_read tcp 5 with 
-  | Correct header ->
-      match Record.parseHeader header with  
-      | Correct (Content.Handshake,pv,len)  ->
-         match really_read tcp len  with
-         | Correct cipher -> 
-	      let payload = decryptRecord_TLS12_AES_GCM_128_SHA256 rd Content.Handshake cipher in
-	      let Correct (rem,hsm) = Handshake.parseHandshakeMessages (Some pv) (Some kex) payload in
-     	      let [(hs_msg,to_log)] = hsm in
-	      hs_msg, log @| to_log	      
-
+  let (Content.Handshake,_,cipher) = recvRecord tcp pv in
+  let payload = decryptRecord_TLS13_AES_GCM_128_SHA256 rd Content.Handshake cipher in
+  let Correct (rem,hsm) = Handshake.parseHandshakeMessages (Some pv) (Some kex) payload in
+  let [(hs_msg,to_log)] = hsm in
+  IO.print_string ("Received HS("^(string_of_handshakeMessage hs_msg)^")\n");
+  hs_msg, log @| to_log	      
 
 let recvEncAppDataRecord tcp pv rd = 
-  match really_read tcp 5 with 
-  | Correct header ->
-      match Record.parseHeader header with  
-      | Correct (Content.Application_data,pv,len)  ->
-         match really_read tcp len  with
-         | Correct cipher -> 
-	      let payload = decryptRecord_TLS12_AES_GCM_128_SHA256 rd Content.Application_data cipher in
-	      payload
+  let (Content.Application_data,_,cipher) = recvRecord tcp pv in
+  let payload = decryptRecord_TLS13_AES_GCM_128_SHA256 rd Content.Application_data cipher in
+  IO.print_string "Received Data:\n";
+  IO.print_string ((iutf8 payload)^"\n");
+  payload
 
-let deriveKeys_TLS12_AES_GCM_128_SHA256 ms cr sr = 
-  let b = TLSPRF.kdf (PRF_TLS_1p2 kdf_label ((HMAC CoreCrypto.SHA256))) ms (sr @| cr) 40 in
-  let cekb, b = split b 16 in
-  let sekb, b = split b 16 in
-  let civb, sivb = split b 4 in
+(* Flex Handshake *)
+
+let deriveKeys_TLS13_AES_GCM_128_SHA256 (secret:bytes) (phase:string) (context:bytes) = 
+  let cekb = HSCrypto.hkdf_expand_label CoreCrypto.SHA256
+      	     secret (phase ^ ", client write key") context 16 in
+  let civb = HSCrypto.hkdf_expand_label CoreCrypto.SHA256
+      	     secret (phase ^ ", client write iv") context 12 in
+  let sekb = HSCrypto.hkdf_expand_label CoreCrypto.SHA256
+      	     secret (phase ^ ", server write key") context 16 in
+  let sivb = HSCrypto.hkdf_expand_label CoreCrypto.SHA256
+      	     secret (phase ^ ", server write iv") context 12 in
   (cekb,civb,sekb,sivb)
 
-    
+let derive_handshake_keys (gxy:CommonDH.secret) (log:bytes) = 
+  let log_hash = CoreCrypto.hash CoreCrypto.SHA256 log in
+  let zeroes = Platform.Bytes.abytes (String.make 32 (Char.char_of_int 0)) in
+  let xES = HSCrypto.hkdf_extract CoreCrypto.SHA256 zeroes gxy in
+  IO.print_string ("zeroes:"^(Platform.Bytes.print_bytes zeroes)^"\n");
+  IO.print_string ("gxy:"^(Platform.Bytes.print_bytes gxy)^"\n");
+  IO.print_string ("xES:"^(Platform.Bytes.print_bytes xES)^"\n");
+  let (ck,civ,sk,siv) = deriveKeys_TLS13_AES_GCM_128_SHA256 xES "handshake key expansion" log_hash in
+  IO.print_string ("client AES_GCM write log_hash:"^(Platform.Bytes.print_bytes log_hash)^"\n");
+  IO.print_string ("client AES_GCM write key:"^(Platform.Bytes.print_bytes ck)^"\n");
+  IO.print_string ("client AES_GCM salt: iv:"^(Platform.Bytes.print_bytes civ)^"\n");
+  IO.print_string ("server AES_GCM write key:"^(Platform.Bytes.print_bytes sk)^"\n");
+  IO.print_string ("server AES_GCM salt:"^(Platform.Bytes.print_bytes siv)^"\n");
+  (ck,civ,sk,siv)
+
 let main host port =
   IO.print_string "===============================================\n Starting test TLS client...\n";
   let tcp = Platform.Tcp.connect host port in
   let log = empty_bytes in
   
-(*
-  let st = Handshake.init Client ... in
-  Handhake.send_client_hello st;
-  let chb = Handshake.next_message st in
-*)
-
-
-  let (Some k,ch,chb) = Handshake.prepareClientHello config None None in
+  let (Some gx,ch,chb) = Handshake.prepareClientHello config None None in
   let pv = ch.ch_protocol_version in 
   let kex = TLSConstants.Kex_ECDHE in
-
-  IO.print_string "Sending ClientHello\n";
-  let log = sendHSRecord tcp pv log chb in
+  let log = sendHSRecord tcp pv (ClientHello ch) log in
 
   let ServerHello(sh),log = recvHSRecord tcp pv kex log in
-  IO.print_string "Received ServerHello\n";
-
+  let Correct (n,ake) = Handshake.processServerHello config None [] ch sh in
   let pv = sh.sh_protocol_version in
   let cs = sh.sh_cipher_suite in
   let CipherSuite kex sa ae = cs in
 
-  let Certificate(sc),log = recvHSRecord tcp pv kex log in
-  IO.print_string "Received ServerCertificate\n";
+  let Some (SEC ec,gyb) = n.n_extensions.ne_keyShare in
+  let Correct gyb = vlparse 1 gyb in 
+  IO.print_string ("server gy:"^(Platform.Bytes.print_bytes gyb)^"\n");
 
+  let Some gyp = ECGroup.parse_point gx.ec_params gyb in  
+  let gy = {ec_params = gx.ec_params; ec_point = gyp; ec_priv = None} in
+  let gxy = CommonDH.dh_initiator (CommonDH.ECKey gx) (CommonDH.ECKey gy) in
+  let (ck,civ,sk,siv) = derive_handshake_keys gxy log in
+  let wr = encryptor_TLS13_AES_GCM_128_SHA256 ck civ in
+  let rd = decryptor_TLS13_AES_GCM_128_SHA256 sk siv in
+
+  let Certificate(sc),log = recvEncHSRecord tcp pv kex log rd in
+
+(*
   let ServerKeyExchange(ske),log = recvHSRecord tcp pv kex log in
-  IO.print_string "Received ServerKeyExchange\n";
-
   let ServerHelloDone,log = recvHSRecord tcp pv kex log in
-  IO.print_string "Received ServerHelloDone\n";
 
   let KEX_S_DHE gy = ske.ske_kex_s in
   let gx, pms = CommonDH.dh_responder gy in
   let cke = {cke_kex_c = kex_c_of_dh_key gx} in
-  let ckeb = clientKeyExchangeBytes sh.sh_protocol_version cke in
-  IO.print_string "Sending ClientKeyExchange\n";
-  let log = sendHSRecord tcp pv log ckeb in
-
+  let log = sendHSRecord tcp pv (ClientKeyExchange cke) log in
+*)
+(*
   let ms = TLSPRF.prf (pv,cs) pms (utf8 "master secret") (ch.ch_client_random @| sh.sh_server_random)  48 in
   IO.print_string ("master secret:"^(Platform.Bytes.print_bytes ms)^"\n");
-
   let (ck,civ,sk,siv) = deriveKeys_TLS12_AES_GCM_128_SHA256 ms ch.ch_client_random sh.sh_server_random in
   IO.print_string ("client AES_GCM write key:"^(Platform.Bytes.print_bytes ck)^"\n");
   IO.print_string ("client AES_GCM salt: iv:"^(Platform.Bytes.print_bytes civ)^"\n");
   IO.print_string ("server AES_GCM write key:"^(Platform.Bytes.print_bytes sk)^"\n");
   IO.print_string ("server AES_GCM salt:"^(Platform.Bytes.print_bytes siv)^"\n");
-  let wr = encryptor_TLS12_AES_GCM_128_SHA256 ck civ in
-  let rd = decryptor_TLS12_AES_GCM_128_SHA256 sk siv in
-
-
-  IO.print_string "Sending ClientCCS\n";
-  sendCCSRecord tcp pv;
 
   let cfin = {fin_vd = TLSPRF.verifyData (pv,cs) ms Client log} in 
-  let cfinb = finishedBytes cfin in
+  let (str,cfinb,log) = makeHSRecord pv (Finished cfin) log in
   let efinb = encryptRecord_TLS12_AES_GCM_128_SHA256 wr Content.Handshake cfinb in
-  IO.print_string "Sending ClientFinished\n";
 
-  let log = sendHSRecord tcp pv log efinb in
+  sendRecord tcp pv Content.Change_cipher_spec HandshakeMessages.ccsBytes "Client";
+  sendRecord tcp pv Content.Handshake efinb str;
 
   let _ = recvCCSRecord tcp pv in
-
-  IO.print_string "Received ServerCCS\n";
   let Finished(sfin),log = recvEncHSRecord tcp pv kex log rd in
-  IO.print_string "Received ServerFinished\n";
 
-  let get = encryptRecord_TLS12_AES_GCM_128_SHA256 wr Content.Application_data (utf8 "GET / HTTP/1.1\r\n\r\n\r\n") in
-  IO.print_string "Sending AppData(GET /)\n";
-  sendAppDataRecord tcp pv get;
+  let payload = "GET / HTTP/1.1\r\nHost: " ^ host ^ "\r\n\r\n" in
+  let get = encryptRecord_TLS12_AES_GCM_128_SHA256 wr Content.Application_data (utf8 payload) in
+
+  sendRecord tcp pv Content.Application_data get "GET /";
   let ad = recvEncAppDataRecord tcp pv rd in
-  IO.print_string "Received AppData:\n";
-  IO.print_string ((iutf8 ad)^"\n");
+*)
   ()
+
   
+
+
+
